%% act-xmod_6.tex  (version 22/04/17) 

\subsection{Semidirect product of crossed modules} 
\label{subs:sdp-xmod}

Just as a group action gives rise to a semidirect product group 
(see subsection \ref{subs:sdp}),
so a crossed module action gives a semidirect product crossed module.

\begin{defn} \label{def:sdp-xmod} 
\index{semidirect product!of crossed modules}
\emph{
The \emph{crossed module semidirect product} 
with $\calY$ acting on $\calX$ is}
$$
\calY \ltimes \calX  \;\;=\;\;
(\,\pi \;:\;Q \ltimes S \,\longrightarrow\, P \ltimes R\,)
$$
\emph{where
\begin{enumerate}[(i)]
\item
$Q \ltimes S$  is the semidirect product with action
$s^q \;=\; s^{\delta q} \;=\; \ddb_{\delta q} s
  \quad \mbox{(see Lemma \ref{lem:ids5}(b) below)}$;
\item
$P \ltimes R$  is the semidirect product with action
$r^p = \db_p r$~;
\item
$\pi(q,s) \;=\; (\delta q,\, \partial s)$~;
\item
$(q,s)^{(p,r)} \;=\; (q^p,\,(\chi_{q^p}\,r)^{-1}\,s^{pr})$~.
\end{enumerate}
}\end{defn}
Note that the action specified in (iv) is a special case of 
Proposition \ref{prop:semidirect-actions}.

\begin{lem}
$\pi$ is a group homomorphism.
\end{lem}
\begin{pf}
\begin{eqnarray*}
\pi(\,(q_1,s_1)(q_2,s_2)\,)  &  =  &
   \pi( q_1q_2,\; {s_1}^{q_2}\,s_2)  \\
 & = &
   (\delta (q_1 q_2),\; 
      \partial(\ddb_{\delta q_2}s_1)(\partial s_2) ) \quad \mbox{by (i)} \\
\pi(q_1,s_1)\;\pi(q_2,s_2)  & = &
   (\delta q_1, \partial s_1)\;(\delta q_2, \partial s_2)  \\
 & = &
   (\,(\delta q_1)(\delta q_2),\;
      (\partial s_1)^{\delta q_2}\,(\partial s_2)\,) \\
 & = &
   (\delta(q_1q_2),\; (\db_{\delta q_2} \partial s_1)\,(\partial s_2)\,)
       \quad \mbox{by (ii)}.
\end{eqnarray*}
and the two right-hand sides are equal since 
$\partial\ddb_p = \db_p\partial \quad \mbox{for all} \;\; p \in P\;$.
\end{pf}


\begin{thm}
The crossed module  $\calY \ltimes \calX$  as defined
\emph{does} satisfy the two crossed modules axioms.
\end{thm}
\begin{pf}
Verification of the first axiom:
\begin{eqnarray*}
(p,r)^{-1}\,\pi(q,s)\,(p,r)
  & = &
   (p,r)^{-1}\,
      (\delta q, \partial s)\,
         (p,r)  \\
  & = &
   (p^{-1},\, (r^{-1})^{p^{-1}})\,
      ((\delta q)p,\, (\partial s)^p\,r\,)  \\
  & = &
   (p^{-1}(\delta q)p,\, 
      (r^{-1})^{p^{-1}(\delta q)p}\,(\partial s)^p\,r\,)  \\
  & = &
   (\,\delta(q^p),\, 
      (r^{\delta q^p})^{-1}\,(\partial s^p)\,r\,)  \\
  & = &
   (\,\delta(q^p),\, 
      (r\,(\partial\chi_{q^p}\,r))^{-1}\,(\partial s^p)\,r\,)
         \hspace{17mm} \mbox{(by \ref{lem:ids5}(c))}  \\
  & = &
   (\,\delta(q^p),\, (\partial\chi_{q^p}\,r)^{-1}\,
       \partial(s^{pr}\,) \\
  & = &
   (\,\delta(q^p),\, \partial( (\chi_{q^p}\,r)^{-1}\, s^{pr} )\,) \\
  & = &
   \pi(\,(q,s)^{(p,r)}\,) ~.
\end{eqnarray*}

\noindent
Verification of the second axiom:
\begin{eqnarray*}\quad
(q,s)^{-1}\,(q_1,s_1)\,(q,s)
  & = &
    (q^{-1},\,((s^{-1})^{q^{-1}})\,(q_1q,\,{s_1}^qs\,)  \\
  & = &
    (\,q^{-1}q_1q,\,(s^{-1})^{q^{-1}q_1q}\,{s_1}^q\,s\,)  \\
  & = &
    (\,{q_1}^{\delta q},\,(s^{-1})^{{q_1}^{\delta q}}\,{s_1}^q\,s\,)\\
  & = &
    (\,{q_1}^{\delta q},\, s^{-1}\,(\chi_{({q_1}^{\delta q})}\,
      (\partial s^{-1}))\,s\,s^{-1}\,
      {s_1}^{(\delta q)}\,s\,) 
         \quad \mbox{(by \ref{lem:ids5}(b))}  \\
  & = &
    (\,{q_1}^{\delta q},\, (\chi_{({q_1}^{\delta q})}\,
      (\partial s^{-1}))^{\partial s}\,
      {s_1}^{(\delta q)(\partial s)}\,) \\
  & = &
    (\,{q_1}^{\delta q},\, (\chi_{({q_1}^{\delta q})}\,\partial s)^{-1}\,
      {s_1}^{(\delta q)(\partial s)}\,) 
         \hspace{19mm} \mbox{(by \ref{lem:invchir}(a))}  \\
  & = &
    (q_1,s_1)^{(\delta q,\,\partial s)}  
         \hspace{48mm} \mbox{(by \ref{def:sdp-xmod}(iv))}  \\
  & = &
    (q_1,s_1)^{\pi(q,s)}
         \hspace{50mm} \mbox{(by \ref{def:sdp-xmod}(iii))} ~. \\
\end{eqnarray*}
\end{pf}

